src/GoSep.v
@@ -1,0 +1,210 @@
+Require Import List FMapAVL Structures.OrderedTypeEx.
+Require Import RelationClasses Morphisms.
+Require Import VerdiTactics.
+Require Import Go.
+
+Set Implicit Arguments.
+Unset Printing Implicit Defensive.
+
+Import Go.
+
+(* TODO What here is actually necessary? *)
+
+Class GoWrapper (WrappedType: Type) :=
+  { wrap:      WrappedType -> Go.value;
+    wrap_inj:  forall v v', wrap v = wrap v' -> v = v' }.
+
+Inductive ScopeItem :=
+| SItem A {H: GoWrapper A} (v : A).
+
+(* None matches nothing *)
+Definition pred := option (VarMap.t ScopeItem).
+
+Definition pred_matches (p : pred) (m : locals) : Prop :=
+  match p with
+    | None => False
+    | Some p' =>
+      forall k item,
+        VarMap.find k p' = Some item ->
+        match item with
+            | SItem val =>
+              VarMap.find k m = Some (wrap val)
+        end
+  end.
+
+Definition pimpl (p q : pred) := forall m, pred_matches p m -> pred_matches q m.
+
+Definition emp : pred := Some (VarMap.empty _).
+
+Definition ptsto var val : pred := Some (VarMap.add var val (VarMap.empty _)).
+
+Module VarMapProperties := FMapFacts.WProperties_fun(Nat_as_OT)(VarMap).
+
+Definition maps_disjoint T (m1 m2 : VarMap.t T) := 
+  VarMapProperties.for_all (fun k1 _ => negb (VarMap.mem k1 m2)) m1.
+
+Lemma for_all_if :
+  forall elt (f : VarMap.key -> elt -> bool),
+    Morphisms.Proper (Morphisms.respectful eq (Morphisms.respectful eq eq)) f ->
+    forall m,
+      VarMapProperties.for_all f m = true ->
+      (forall k e, VarMap.MapsTo k e m -> f k e = true).
+Proof.
+  firstorder using VarMapProperties.for_all_iff.
+Qed.
+
+Lemma maps_disjoint_comm :
+  forall T m1 m2, @maps_disjoint T m1 m2 = maps_disjoint m2 m1.
+Proof.
+  unfold maps_disjoint.
+  intros.
+  match goal with
+    | [ |- context[VarMapProperties.for_all ?p m1] ] => case_eq (VarMapProperties.for_all p m1)
+  end;
+  match goal with
+    | [ |- context[VarMapProperties.for_all ?p m2] ] => case_eq (VarMapProperties.for_all p m2)
+  end; try congruence; intros; exfalso.
+Admitted.
+
+Definition sep_star_impl (p1 p2 : pred) : pred :=
+  match p1, p2 with
+    | Some m1, Some m2 =>
+      if maps_disjoint m1 m2
+      then Some (VarMapProperties.update m1 m2)
+      else None
+    | _, _ => None
+  end.
+
+Module Type SEP_STAR.
+  Parameter sep_star : pred -> pred -> pred.
+  Axiom sep_star_is : @sep_star = @sep_star_impl.
+End SEP_STAR.
+
+Module Sep_Star : SEP_STAR.
+  Definition sep_star := @sep_star_impl.
+  Theorem sep_star_is : @sep_star = @sep_star_impl.
+  Proof. auto. Qed.
+End Sep_Star.
+
+Definition sep_star := @Sep_Star.sep_star.
+Definition sep_star_is := Sep_Star.sep_star_is.
+
+Infix "|->" := ptsto (at level 35) : go_pred_scope.
+Bind Scope go_pred_scope with pred.
+
+Delimit Scope go_pred_scope with go_pred.
+
+Notation "k ~> v" := (k |-> (SItem v))%go_pred (at level 35) : go_pred_scope.
+
+Infix "*" := sep_star : go_pred_scope.
+Notation "∅" := emp : go_pred_scope.
+Notation "p =p=> q" := (pimpl p%go_pred q%go_pred) (right associativity, at level 60) : go_pred_scope.
+Notation "m ## p" := (pred_matches p%go_pred m) (at level 70).
+
+Local Open Scope go_pred.
+
+Ltac unfold_sep_star := unfold sep_star; rewrite sep_star_is; unfold sep_star_impl.
+
+Theorem sep_star_comm :
+  forall p1 p2,
+    p1 * p2 =p=> p2 * p1.
+Proof.
+  unfold pimpl, pred_matches.
+  unfold_sep_star.
+  intros.
+  destruct p1, p2; eauto.
+  rewrite maps_disjoint_comm.
+  case_eq (maps_disjoint t t0); intro He; rewrite ?He in *; auto; intros.
+  destruct item.
+  eapply VarMap.find_1.
+  find_eapply_lem_hyp VarMap.find_2.
+  pose proof (VarMapProperties.update_mapsto_iff t t0 k (SItem v)).
+  pose proof (VarMapProperties.update_mapsto_iff t0 t k (SItem v)).
+Admitted.
+
+Theorem sep_star_assoc_1 :
+  forall p1 p2 p3,
+    p1 * p2 * p3 =p=> p1 * (p2 * p3).
+Proof.
+Admitted.
+
+Theorem sep_star_assoc_2 :
+  forall p1 p2 p3,
+    p1 * (p2 * p3) =p=> p1 * p2 * p3.
+Proof.
+Admitted.
+
+Theorem pimpl_refl :
+  forall p, p =p=> p.
+Admitted.
+
+Theorem pimpl_trans :
+  forall p q r,
+    p =p=> q ->
+    q =p=> r ->
+    p =p=> r.
+Admitted.
+
+Theorem pimpl_apply :
+  forall p q m,
+    p =p=> q ->
+    m ## p ->
+    m ## q.
+Proof.
+  intros.
+Admitted.
+
+Theorem pimpl_l :
+  forall p q,
+    p * q =p=> p.
+Admitted.
+
+Theorem pimpl_r :
+  forall p q,
+    p * q =p=> q.
+Admitted.
+
+Theorem emp_l_1 :
+  forall p,
+    p =p=> p * emp.
+Admitted.
+
+Theorem emp_l_2 :
+  forall p,
+    p * emp =p=> p.
+Admitted.
+
+Theorem ptsto_find :
+  forall A {H : GoWrapper A} k (v : A) F m,
+    m ## k ~> v * F ->
+    VarMap.find k m = Some (wrap v).
+Proof.
+  unfold pred_matches, ptsto.
+  unfold_sep_star.
+  intros.
+  break_match; intuition.
+Admitted.
+
+Theorem ptsto_update :
+  forall A {H : GoWrapper A} k (v : A) F m,
+    m ## F ->
+    VarMap.add k (wrap v) m ## k ~> v * F.
+Admitted.
+
+Instance pimpl_preorder :
+  PreOrder pimpl.
+Proof.
+  split.
+  exact pimpl_refl.
+  exact pimpl_trans.
+Qed.
+
+Instance pred_apply_pimpl_proper :
+  Proper (pimpl ==> eq ==> Basics.impl) pred_matches.
+Proof.
+  unfold pimpl, pred_matches.
+  intros p q Hpq ma mb Hmab H.
+  destruct p, q; intuition subst.
+  eapply Hpq; eauto.
+  apply Hpq in H; trivial.
+Qed.
